theories/iris/examples/stack/stack_instantiation_interp.v
@@ -1,0 +1,287 @@
+From mathcomp Require Import ssreflect eqtype seq ssrbool.
+From iris.program_logic Require Import language.
+From iris.proofmode Require Import base tactics classes.
+From iris.base_logic Require Export gen_heap ghost_map proph_map na_invariants.
+From iris.base_logic.lib Require Export fancy_updates.
+From iris.bi Require Export weakestpre.
+Require Export iris iris_locations iris_properties iris_atomicity stdpp_aux.
+Require Export iris_host iris_fundamental_helpers stack_specs stack_instantiation.
+Require Export datatypes operations properties opsem.
+
+Set Implicit Arguments.
+Unset Strict Implicit.
+Unset Printing Implicit Defensive.
+
+Close Scope byte_scope.
+
+Section StackModule.
+  Context `{!wasmG Σ, !hvisG Σ, !hmsG Σ, !hasG Σ}.
+
+  Set Bullet Behavior "Strict Subproofs".
+
+  Definition stack_t_context :=
+  {| tc_types_t := [Tf [] [T_i32]; Tf [T_i32] [T_i32]; Tf [T_i32; T_i32] []];
+    tc_func_t := [Tf [] [T_i32]; Tf [T_i32] [T_i32]; Tf [T_i32] [T_i32]; Tf [T_i32] [T_i32]; Tf [T_i32; T_i32] []; Tf [T_i32; T_i32] []];
+    tc_global := [];
+    tc_table := [ {| tt_limits := {| lim_min := 1; lim_max := None |}; tt_elem_type := ELT_funcref |}];
+    tc_memory := [ {| lim_min := 0; lim_max := None |}];
+    tc_local := [];
+    tc_label := [];
+    tc_return := None
+  |}.
+  
+  Lemma instantiate_stack_spec `{!logrel_na_invs Σ} (s : stuckness) (E: coPset) (hv0 hv1 hv2 hv3 hv4 hv5 hv6 : module_export) :
+  (* Knowing 0%N holds the stack module… *)
+  0%N ↪[mods] stack_module -∗
+     (* … and we own the vis 0%N thru 4%N … *)
+     ([∗ list] k↦hvk ∈ [hv0 ; hv1 ; hv2 ; hv3 ; hv4 ; hv5 ; hv6], N.of_nat k ↪[vis] hvk) -∗
+     (* … instantiating the stack-module (by lazyness, this is expressed here with
+        a take 1 in order to avoir rewriting the instantiation), yields the following : *)
+     WP ((stack_instantiate, []) : host_expr)
+     @ s ; E
+             {{ λ v : host_val,
+                 (* Instantiation succeeds *)
+                 ⌜ v = immHV [] ⌝ ∗
+                 (* 0%N still owns the stack_module *)
+                 0%N ↪[mods] stack_module ∗ 
+                  ∃ (idf0 idf1 idf2 idf3 idf4 idf5 idt : nat)
+                    (name0 name1 name2 name3 name4 name5 name6 : name)
+                    (f0 f1 f2 f3 f4 f5 : list basic_instruction)
+                    (i0 : instance)
+                    (l0 l1 l2 l3 l4 l5 : list value_type)
+                    tab 
+                    (isStack : Z -> seq.seq i32 -> iPropI Σ)
+                    (nextStackAddrIs : nat -> iPropI Σ), 
+                    (* Our exports are in the vis 0%N thru 4%N. Note that everything is 
+                       existantially quantified. In fact, all the f_i, i_i and l_i 
+                       could be given explicitely, but we quantify them existantially 
+                       to show modularity : we do not care what the functions are, 
+                       we only care about their spec (see next comment). This also
+                       makes this lemma more readable than if we stated explicitely all
+                       the codes of the functions *)
+                    let inst_vis := (map (λ '(name, idf),
+                                                 {| modexp_name := name ;
+                                                   modexp_desc := MED_func (Mk_funcidx idf)
+                                                 |}) [(name0, idf0) ; (name1, idf1) ;
+                                                      (name2, idf2) ; (name3, idf3) ;
+                                                      (name4, idf4) ; (name5, idf5) ])
+                                        ++ [ {| modexp_name := name6 ;
+                                               modexp_desc := MED_table (Mk_tableidx idt) |} ]
+                    in 
+                    let inst_map := fold_left (λ fs '(idf,i,t,l,f),
+                                                <[ N.of_nat idf := FC_func_native i t l f ]> fs)
+                                              (rev [(idf0, i0, Tf [] [T_i32], l0, f0) ;
+                                               (idf1, i0, Tf [T_i32] [T_i32], l1, f1) ;
+                                                    (idf2, i0, Tf [T_i32] [T_i32], l2, f2) ;
+                                                    (idf3, i0, Tf [T_i32] [T_i32], l3, f3) ;
+                                                    (idf4, i0, Tf [T_i32 ; T_i32] [], l4, f4) ;
+                                              (idf5, i0, Tf [T_i32 ; T_i32] [], l5, f5)])
+                                              ∅ in
+                    let tab_data := tab.(table_data) in
+                    let tab_size := length tab_data in
+                    (* These two import functions state that all [vis] and [wf] point 
+                       to the correct exports/functions, i.e. a client will be able 
+                       to successfully import them *)
+                    import_resources_host [0%N; 1%N; 2%N; 3%N; 4%N ; 5%N ; 6%N] inst_vis ∗
+                    import_resources_wasm_typecheck_sepL2 inst_vis expts inst_map
+                    (<[ N.of_nat idt := tab ]> ∅) 
+                    ∅ ∅ ∗
+                    ⌜ NoDup (modexp_desc <$> inst_vis) ⌝ ∗
+                    ⌜ tab_size >= 1 ⌝ ∗
+                    na_inv logrel_nais stkN (stackModuleInv isStack nextStackAddrIs) ∗
+                    (* table starts out as empty *)
+                    ([∗ list] elem ∈ tab_data, ⌜elem = None⌝) ∗
+                    (* each export function is valid *)
+                    [∗ map] f↦cl ∈ inst_map, interp_closure [] (cl_type cl) cl
+             }}.
+  Proof.
+    iIntros "Hmod (Hhv0 & Hhv1 & Hhv2 & Hhv3 & Hhv4 & Hhv5 & Hhv6 & _)".
+    iApply (weakestpre.wp_strong_mono s _ E
+             with "[Hmod Hhv0 Hhv1 Hhv2 Hhv3 Hhv4 Hhv5 Hhv6]") => //.
+    iApply (instantiation_spec_operational_no_start
+             with "[Hmod Hhv0 Hhv1 Hhv2 Hhv3 Hhv4 Hhv5 Hhv6]") ;
+      try exact module_typing_stack => //.
+    - by unfold stack_module.
+    - unfold module_restrictions => /=.
+      repeat split => //=.
+      exists [] => //.
+      exists [] => //.
+      exists [] => //.
+    - unfold instantiation_resources_pre.
+      iSplitL "Hmod" ; first done.
+      unfold instantiation_resources_pre_wasm.
+      rewrite irwt_nodup_equiv.
+      repeat iSplit.
+      + by unfold import_resources_host.
+      + iPureIntro. apply dom_empty.
+      + iPureIntro. apply dom_empty.
+      + iPureIntro. apply dom_empty.
+      + iPureIntro. apply dom_empty.
+      + done.
+      + iPureIntro. unfold module_elem_bound_check_gmap => //=.
+      + iPureIntro. unfold module_data_bound_check_gmap => //=.
+      + unfold export_ownership_host.
+        iSplitL "Hhv0".
+        by iExists _.
+        iSplitL "Hhv1".
+        by iExists _.
+        iSplitL "Hhv2".
+        by iExists _.
+        iSplitL "Hhv3".
+        by iExists _.
+        iSplitL "Hhv4".
+        by iExists _.
+        iSplitL "Hhv5".
+        by iExists _.
+        iSplitL "Hhv6".
+        by iExists _.
+        done.
+      + done.
+      + simpl. by apply NoDup_nil.
+    - iIntros (v) "Hinst".
+      unfold instantiation_resources_post.
+      iDestruct "Hinst" as "(%Hvsucc & Hmod & Himphost & Hinst)".
+      subst v; iSplitR => //.
+      iDestruct "Hinst" as (inst) "[Himpwasm Hexphost]".
+      iDestruct "Himpwasm" as (g_inits t_inits m_inits gms wts wms) "(Himpwasm & %Hinst & -> & -> & %Hbound & -> & -> & %Hbound' & %Hginit & -> & Hexpwasm)".
+      destruct Hinst as (Hinsttype & Hinstfunc & Hinsttab & Hinstmem & Hinstglob).
+      unfold module_inst_resources_wasm, module_export_resources_host => /=.
+      destruct inst => /=.
+      iDestruct "Hexpwasm" as "(Hexpwf & Hexpwt & Hexpwm & Hexpwg)".
+      unfold module_inst_resources_func, module_inst_resources_glob,
+        module_inst_resources_tab, module_inst_resources_mem => /=.
+      unfold big_sepL2 => /=.
+      destruct inst_funcs as [|? inst_funcs] ; first done ;
+        iDestruct "Hexpwf" as "[Hf Hexpwf]".
+      destruct inst_funcs as [|? inst_funcs] ; first done ;
+        iDestruct "Hexpwf" as "[Hf0 Hexpwf]".
+      destruct inst_funcs as [|? inst_funcs] ; first done ;
+        iDestruct "Hexpwf" as "[Hf1 Hexpwf]".
+      destruct inst_funcs as [|? inst_funcs] ; first done ;
+        iDestruct "Hexpwf" as "[Hf2 Hexpwf]".
+      destruct inst_funcs as [|? inst_funcs] ; first done ;
+        iDestruct "Hexpwf" as "[Hf3 Hexpwf]".
+      destruct inst_funcs as [| ? inst_funcs] ; first done ;
+        iDestruct "Hexpwf" as "[Hf4 Hexpwf]".
+      destruct inst_funcs ; last done.
+      destruct inst_tab ; first done.
+      iDestruct "Hexpwt" as "[Htab Hexpwt]".
+      destruct inst_tab ; last done.
+      destruct inst_memory as [|m inst_memory] ; first done.
+      iDestruct "Hexpwm" as "[Hexpwm ?]".
+      destruct inst_memory ; last done.
+      iDestruct "Hexpwm" as "(Hexpwm & Hmemlength & Hmemlim)".
+      destruct inst_globs ; last done.
+      iDestruct "Hexphost" as "(Hexp0 & Hexp1 & Hexp2 & Hexp3 & Hexp4 & Hexp5 & Hexp6 & _)".
+      iDestruct "Hexp0" as (name0) "Hexp0".
+      iDestruct "Hexp1" as (name1) "Hexp1".
+      iDestruct "Hexp2" as (name2) "Hexp2".
+      iDestruct "Hexp3" as (name3) "Hexp3".
+      iDestruct "Hexp4" as (name4) "Hexp4".
+      iDestruct "Hexp5" as (name5) "Hexp5".
+      iDestruct "Hexp6" as (name6) "Hexp6".
+      simpl in * ; subst.
+      iSplitL "Hmod" ; first done.
+      iExists f, f0, f1, f2, f3, f4, t.
+      iExists name0, name1, name2, name3, name4, name5, name6.
+      iExists _, _, _, _, _, _.
+      iExists _.
+      iExists _, _, _, _, _, _.
+      iExists _.
+      iExists (λ a b, isStack a b m).
+      iExists (λ n, (N.of_nat m↦[wmlength] N.of_nat n)%I).
+      iDestruct (mapsto_frac_ne with "Hf Hf0") as "%H01" ; first by eauto.
+      iDestruct (mapsto_frac_ne with "Hf Hf1") as "%H02" ; first by eauto.
+      iDestruct (mapsto_frac_ne with "Hf Hf2") as "%H03" ; first by eauto.
+      iDestruct (mapsto_frac_ne with "Hf Hf3") as "%H04" ; first by eauto.
+      iDestruct (mapsto_frac_ne with "Hf Hf4") as "%H05" ; first by eauto.
+      iDestruct (mapsto_frac_ne with "Hf0 Hf1") as "%H12" ; first by eauto.
+      iDestruct (mapsto_frac_ne with "Hf0 Hf2") as "%H13" ; first by eauto.
+      iDestruct (mapsto_frac_ne with "Hf0 Hf3") as "%H14" ; first by eauto.
+      iDestruct (mapsto_frac_ne with "Hf0 Hf4") as "%H15" ; first by eauto.
+      iDestruct (mapsto_frac_ne with "Hf1 Hf2") as "%H23" ; first by eauto.
+      iDestruct (mapsto_frac_ne with "Hf1 Hf3") as "%H24" ; first by eauto.
+      iDestruct (mapsto_frac_ne with "Hf1 Hf4") as "%H25" ; first by eauto.
+      iDestruct (mapsto_frac_ne with "Hf2 Hf3") as "%H34" ; first by eauto.
+      iDestruct (mapsto_frac_ne with "Hf2 Hf4") as "%H35" ; first by eauto.
+      iDestruct (mapsto_frac_ne with "Hf3 Hf4") as "%H45" ; first by eauto.
+      iSplitL "Hexp0 Hexp1 Hexp2 Hexp3 Hexp4 Hexp5 Hexp6".
+      unfold import_resources_host.
+      iFrame. by iModIntro.
+      iSplitL "Hf Hf0 Hf1 Hf2 Hf3 Hf4 Htab".
+      iSplitR.
+      + iPureIntro.
+        simpl.
+        repeat rewrite dom_insert.
+        done.
+      + iSplitL "Hf".
+        iExists _.
+        iFrame.
+        iPureIntro.
+        rewrite lookup_insert.
+        split => //.
+        iSplitL "Hf0".
+        iExists _ ; iFrame.
+        iPureIntro.
+        rewrite lookup_insert_ne ; last assumption.
+        rewrite lookup_insert.
+        split => //.
+        iSplitL "Hf1".
+        iExists _ ; iFrame.
+        iPureIntro.
+        do 2 (rewrite lookup_insert_ne ; last assumption).
+        rewrite lookup_insert.
+        split => //.
+        iSplitL "Hf2".
+        iExists _ ; iFrame.
+        iPureIntro.
+        do 3 (rewrite lookup_insert_ne ; last assumption).
+        rewrite lookup_insert.
+        split => //.
+        iSplitL "Hf3".
+        iExists _ ; iFrame.
+        iPureIntro.
+        do 4 (rewrite lookup_insert_ne ; last assumption).
+        rewrite lookup_insert.
+        split => //.
+        iSplitL "Hf4".
+        iExists _ ; iFrame.
+        iPureIntro.
+        do 5 (rewrite lookup_insert_ne ; last assumption).
+        rewrite lookup_insert.
+        split => //.
+        iSplitL; cbn; last done.
+        iExists _, _ ; iFrame.
+        iPureIntro.
+        rewrite lookup_insert.
+        split => //.
+      + iSplitR.
+        { iPureIntro.
+          repeat (apply NoDup_cons; split; cbn; first by set_solver).
+          by apply NoDup_nil.
+        }
+        iSplitR.
+        iPureIntro.
+        simpl.
+        lia.
+
+        iMod (na_inv_alloc logrel_nais _ stkN (stackModuleInv _ (λ n : nat, N.of_nat m↦[wmlength]N.of_nat n)%I) with "[Hmemlength]") as "#Hstk".
+        { iNext. iExists 0. iSplit.
+          - iPureIntro. apply PeanoNat.Nat.divide_0_r.
+          - iFrame. iIntros (? [? ?]). exfalso. lia. }
+        iFrame "Hstk". iClear "∗".
+        set (i0 := {| inst_types := [Tf [] [T_i32]; Tf [T_i32] [T_i32]; Tf [T_i32; T_i32] []];
+                     inst_funcs := [f; f0; f1; f2; f3; f4];
+                     inst_tab := [t];
+                     inst_memory := [m];
+                     inst_globs := []
+                   |}).
+        iSplitR;[simpl;auto|].
+        repeat (rewrite big_sepM_insert;[|simplify_map_eq; done]).
+        repeat iSplitR;iModIntro;[..|iApply big_sepM_empty;done];auto;iModIntro;iNext.
+        * 
+        
+        
+    
+
+End StackModule.
