theories/iris/examples/stack/stack_module_robust.v
@@ -1,0 +1,117 @@
+From mathcomp Require Import ssreflect eqtype seq ssrbool.
+From iris.program_logic Require Import language.
+From iris.proofmode Require Import base tactics classes.
+From iris.base_logic Require Export gen_heap ghost_map proph_map na_invariants.
+From iris.base_logic.lib Require Export fancy_updates.
+From iris.bi Require Export weakestpre.
+Require Export iris iris_locations iris_properties iris_atomicity stdpp_aux.
+Require Export iris_host iris_fundamental_helpers stack_specs stack_instantiation iris_interp_instance_alloc proofmode.
+Require Export iris_example_helper.
+Require Export datatypes operations properties opsem.
+
+Set Implicit Arguments.
+Unset Strict Implicit.
+Unset Printing Implicit Defensive.
+
+Close Scope byte_scope.
+   
+
+Section RobustStack.
+  Context `{!wasmG Σ, !hvisG Σ, !hmsG Σ,
+      !logrel_na_invs Σ, !hasG Σ}.
+
+  Notation "{{{ P }}} es {{{ v , Q }}}" :=
+    (□ ∀ Φ, P -∗ (∀ v, Q -∗ Φ v) -∗ WP (es : host_expr) @ NotStuck ; ⊤ {{ v, Φ v }})%I (at level 50).
+  
+  Definition stack_adv_instantiate :=
+    [ ID_instantiate [0%N ; 1%N ; 2%N ; 3%N ; 4%N ; 5%N ; 6%N] 0 [] ;
+      ID_instantiate [] 1 [0%N ; 1%N ; 2%N ; 3%N ; 4%N ; 5%N ; 6%N] ].
+
+  Definition stack_module_imports := expts.
+
+  Lemma instantiate_stack_adv_spec adv_module start :
+    module_typing adv_module expts [] -> (* we assume the adversary module imports the stack module) *)
+    mod_start adv_module = Some start -> (* that it does have a start function *)
+    module_restrictions adv_module -> (* that it adheres to the module restrictions (i.e. only constant initializers for globals) *)
+    module_elem_bound_check_gmap ∅ [] adv_module -> (* if the adversary module declares a table, there cannot be more initializers that its size *)
+    module_data_bound_check_gmap ∅ [] adv_module -> (* if the adversary module declares a memory, there cannot be more initializers that its size *)
+
+    ⊢ {{{ 0%N ↪[mods] stack_module ∗
+          1%N ↪[mods] adv_module ∗
+          na_own logrel_nais ⊤ ∗
+          (∃ vs0 vs1 vs2 vs3 vs4 vs5 vs6, [∗ list] v↦vs∈[vs0;vs1;vs2;vs3;vs4;vs5;vs6], N.of_nat v ↪[vis] vs) ∗
+          ↪[frame] empty_frame
+      }}}
+        ((stack_adv_instantiate,[]) : host_expr) 
+      {{{ v, True }}} .
+  Proof.
+    iIntros (Htyp Hnostart Hrestrict Hboundst Hboundsm).
+    iModIntro. iIntros (Φ) "(Hmod_stack & Hmod_adv & Hown & 
+                        Hvisvst & Hemptyframe) HΦ".
+    iDestruct "Hvisvst" as (vs0 vs1 vs2 vs3 vs4 vs5 vs6) "Hvis".
+
+    (* instantiate stack module *)
+    iApply (wp_seq_host_nostart NotStuck with "[] [$Hmod_stack] [Hvis] ") => //.
+    2: { iIntros "Hmod_stack".
+      iApply weakestpre.wp_mono;cycle 1.
+      iApply (instantiate_stack_spec with "[$]").
+      { iFrame "Hvis". }
+      iIntros (v) "[Hvsucc [$ Hv]]".
+      iCombine "Hvsucc Hv" as "Hv".
+      iExact "Hv". }
+    { by iIntros "(% & ?)". }
+    iIntros (w) "Hstack Hmod_stack".
+
+    iDestruct "Hstack" as "(-> & Hstack)".
+    
+    iDestruct "Hstack" as (idf0 idf1 idf2 idf3 idf4 idf5 idt) "Hstack".
+    iDestruct "Hstack" as (nm0 nm1 nm2 nm3 nm4 nm5 nm6 f0 f1 f2) "Hstack".
+    iDestruct "Hstack" as (f3 f4 f5 istack l0 l1 l2 l3 l4 l5) "Hstack".
+    iDestruct "Hstack" as (stacktab isStack newStackAddrIs) "Hstack".
+    iDestruct "Hstack" as "(HimpsH & HimpsW & %Hnodup & %Htablen & HnewStackAddrIs 
+    & #Hnewstack & #Hisempty & #Hisfull & #Hpop & #Hpush & #Hmap & #Hmaptrap) /=".
+    
+    (* Cleanup of stack resources *)
+    iDestruct "HimpsW" as "(_ & Hidf0 & Hidf1 & Hidf2 & Hidf3 & Hidf4 & Hidf5 & Hidtab & _) /=".
+     repeat (rewrite lookup_insert + (rewrite lookup_insert_ne;[|done])).
+    iDestruct "Hidf0" as (cl0) "[Himpfcl0 Hcl0]".
+    iDestruct "Hidf1" as (cl1) "[Himpfcl1 Hcl1]".
+    iDestruct "Hidf2" as (cl2) "[Himpfcl2 Hcl2]".
+    iDestruct "Hidf3" as (cl3) "[Himpfcl3 Hcl3]".
+    iDestruct "Hidf4" as (cl4) "[Himpfcl4 Hcl4]".
+    iDestruct "Hidf5" as (cl5) "[Himpfcl5 Hcl5]".
+    iDestruct (mapsto_frac_ne with "Himpfcl0 Himpfcl1") as "%H01" ; first by eauto.
+    iDestruct (mapsto_frac_ne with "Himpfcl0 Himpfcl2") as "%H02" ; first by eauto.
+    iDestruct (mapsto_frac_ne with "Himpfcl0 Himpfcl3") as "%H03" ; first by eauto.
+    iDestruct (mapsto_frac_ne with "Himpfcl0 Himpfcl4") as "%H04" ; first by eauto.
+    iDestruct (mapsto_frac_ne with "Himpfcl0 Himpfcl5") as "%H05" ; first by eauto.
+    iDestruct (mapsto_frac_ne with "Himpfcl1 Himpfcl2") as "%H12" ; first by eauto.
+    iDestruct (mapsto_frac_ne with "Himpfcl1 Himpfcl3") as "%H13" ; first by eauto.
+    iDestruct (mapsto_frac_ne with "Himpfcl1 Himpfcl4") as "%H14" ; first by eauto.
+    iDestruct (mapsto_frac_ne with "Himpfcl1 Himpfcl5") as "%H15" ; first by eauto.
+    iDestruct (mapsto_frac_ne with "Himpfcl2 Himpfcl3") as "%H23" ; first by eauto.
+    iDestruct (mapsto_frac_ne with "Himpfcl2 Himpfcl4") as "%H24" ; first by eauto.
+    iDestruct (mapsto_frac_ne with "Himpfcl2 Himpfcl5") as "%H25" ; first by eauto.
+    iDestruct (mapsto_frac_ne with "Himpfcl3 Himpfcl4") as "%H34" ; first by eauto.
+    iDestruct (mapsto_frac_ne with "Himpfcl3 Himpfcl5") as "%H35" ; first by eauto.
+    iDestruct (mapsto_frac_ne with "Himpfcl4 Himpfcl5") as "%H45" ; first by eauto.
+    repeat (rewrite lookup_insert + (rewrite lookup_insert_ne;[|done])).
+    iDestruct "Hcl0" as %[Heq1 Heq2];inversion Heq1;inversion Heq2;clear Heq1 Heq2.
+    iDestruct "Hcl1" as %[Heq1 Heq2];inversion Heq1;inversion Heq2;clear Heq1 Heq2.
+    iDestruct "Hcl2" as %[Heq1 Heq2];inversion Heq1;inversion Heq2;clear Heq1 Heq2.
+    iDestruct "Hcl3" as %[Heq1 Heq2];inversion Heq1;inversion Heq2;clear Heq1 Heq2.
+    iDestruct "Hcl4" as %[Heq1 Heq2];inversion Heq1;inversion Heq2;clear Heq1 Heq2.
+    iDestruct "Hcl5" as %[Heq1 Heq2];inversion Heq1;inversion Heq2;clear Heq1 Heq2.
+    subst cl0 cl1 cl2 cl3 cl4 cl5.
+    iDestruct "Hidtab" as (tab tt) "[Hidtab [%Heq %Htt]]". inversion Heq;subst tab.
+    clear H01 H02 H03 H04 H05 H12 H13 H14 H15 H23 H24 H25 H34 H35 H45 H1 H3 H5 H7 H9 H11.
+    iDestruct "HimpsH" as "(Hvis0 & Hvis1 & Hvis2 & Hvis3 & Hvis4 & Hvis5 & Hvis6 & _)".
+
+    (* instantiate adversary module *)
+
+    (* first we must establish the validity of each import object *)
+    
+
+    
+
+End RobustStack.
